\item Find a transformation matrix $\mathbf{S}$ such that
\begin{equation*}
 \mathbf{S}^{-1} \mathbf{A} \mathbf{S} = \mathbf{J}
\end{equation*}
where
\begin{equation*}
 \mathbf{A} = \begin{bmatrix}
      4 & 1 & -2\\
      1 & 0 & 2\\
      1 & -1 & 3
     \end{bmatrix}
, \qquad
\mathbf{J} = \begin{bmatrix}
     3 & 1 & 0\\
     0 & 3 & 0\\
     0 & 0 & 1
    \end{bmatrix}
\end{equation*}

We first obtain the eigenvalues of the matrix.

\begin{align*}
 \Delta (\lambda) &=
 \det (\lambda \mathbf{I} - \mathbf{A}) = 0\\
 &=  \det \left (
 \begin{bmatrix}
  \lambda -4 & -1 & 2\\
  -1 & \lambda & -2\\
  -1 & 1 & \lambda -3
 \end{bmatrix}
 \right)
\end{align*}

\begin{equation*}
 \lambda = 3 \quad \lambda = 3 \quad \lambda = 1
\end{equation*}

Due to the repeated roots, it is necessary to
construct generalized eignevectors to form $\mathbf{S}$.

We obtain the basis.

\begin{align*}
 (\mathbf{A}-\lambda\mathbf{I}) &= \begin{bmatrix}
                                    4-\lambda & 1 & -2\\
                                    1 & -\lambda &2\\
                                    1 & -1 & 3 -\lambda
                                   \end{bmatrix}
\\
 \lambda = 1 & \rightarrow (\mathbf{A}-\lambda\mathbf{I}) = \begin{bmatrix}
                                    3 & 1 & -2\\
                                    1 & -1 &2\\
                                    1 & -1 & 2
                                   \end{bmatrix}
\\
 \lambda = 3 & \rightarrow (\mathbf{A}-\lambda\mathbf{I}) = \begin{bmatrix}
                                      1 & 1 & -2\\
                                      1 & -3 & 2\\
                                      1 & -1 & 0
                                     \end{bmatrix}\\
& \rightarrow (\mathbf{A}-\lambda\mathbf{I})^2 = \begin{bmatrix}
                                      0 & 0 & 0\\
                                      0 & 8 &-8\\
                                      0 & 4 & -4
                                     \end{bmatrix}
\end{align*}

Find a solution to
\begin{align*}
(\mathbf{A}- \mathbf{I}) \mathbf{v}_3& = \mathbf{0} \\
(\mathbf{A}-3 \mathbf{I})^2 \mathbf{v}_2 & = \mathbf{0} \\
(\mathbf{A}- 3\mathbf{I}) \mathbf{v}_2& = \mathbf{v}_1 \\
\end{align*}

\begin{align*}
 (\mathbf{A}- \mathbf{I}) \mathbf{v}_3& = \mathbf{0} \\
 (\mathbf{A}-\lambda \mathbf{I}) = \begin{bmatrix}
                                    3 & 1 & -2\\
                                    1 & -1 &2\\
                                    1 & -1 & 2
 \end{bmatrix}
&\rightarrow \mathbf{v}_3= \begin{bmatrix}
                            0\\2\\1
                           \end{bmatrix}
\end{align*}
% A^2
\begin{align*}
 (\mathbf{A}-3 \mathbf{I})^2 \mathbf{v}_2 & = \mathbf{0} \\
 (\mathbf{A}-\lambda \mathbf{I})^2 = \begin{bmatrix}
  0 & 0 & 0\\
                                      0 & 8 & -8\\
                                      0 & 4 & -4
 \end{bmatrix}
&\rightarrow \mathbf{v}_2= \begin{bmatrix}
                            1\\0\\0
                           \end{bmatrix}
\end{align*}
% A
\begin{align*}
 (\mathbf{A}- 3\mathbf{I}) \mathbf{v}_2& = \mathbf{v}_1 \\
 (\mathbf{A}-\lambda \mathbf{I}) = \begin{bmatrix}
  1 & 1 & -2\\
                                    1 & -3 &2\\
                                    1 & -1 & 0
 \end{bmatrix}
&\rightarrow \mathbf{v}_1= \begin{bmatrix}
                            1\\1\\1
                           \end{bmatrix}
\end{align*}

 Thus the Jordan form is

 \begin{align*}
 \mathbf{J} &= \begin{bmatrix}
                       3 & 1 & 0\\ 0&3&0\\0&0&1
                      \end{bmatrix}\\
  \mathbf{S} &= \begin{bmatrix}
   1 & 1 & 0\\
   1 & 0 & 2\\
   1 & 0 & 1
  \end{bmatrix}
 \end{align*}




